

$$\begin{aligned}
 1) \quad \frac{\frac{2}{7} - \frac{2}{5}}{\frac{-\frac{1}{3} - \frac{1}{6}}{2}} &= \frac{\frac{10-21}{35}}{\frac{-2-1}{6}} = \frac{-\frac{11}{35}}{-\frac{1}{2}} \\
 &= \frac{-\frac{11}{35}}{-\frac{1}{2} \cdot \frac{1}{2}} = + \frac{11}{35} \cdot \frac{4}{1} = \frac{44}{35}
 \end{aligned}$$

$$\frac{20}{60} = \boxed{\frac{1}{3}}$$

$$2) \quad \frac{\frac{\sqrt{x+y}}{\sqrt{x-y}}}{\frac{x^2-y^2}{\sqrt{x+y}}} - x - y = \frac{\sqrt{x+y}}{\frac{\sqrt{x-y}}{\sqrt{x+y} \sqrt{x-y}}} - x - y$$

$$A^2 - B^2 = (A+B)(A-B)$$

$$\sqrt[n]{a \cdot b} = \sqrt[n]{a} \cdot \sqrt[n]{b}$$

$$= \frac{\sqrt{x+y}}{\frac{1}{\sqrt{x+y}}} - x - y = (\sqrt{x+y})^2 - x - y$$

$$\begin{aligned}
 &= x + y - x - y \\
 &= \textcircled{0}
 \end{aligned}$$

$$\begin{aligned}
 &x^2 - y^2 \neq 0 \\
 &\swarrow \\
 &x - y \neq 0 \\
 &\downarrow \\
 &(x+y) \cdot (x-y) \neq 0
 \end{aligned}$$

$$\boxed{
 \begin{array}{ll}
 x \neq \pm y & x+y > 0 \\
 & x-y > 0
 \end{array}
 }$$

$$3) 5 \sqrt{\left(\frac{c^{\frac{1}{2}} \cdot c^{-\frac{1}{3}}}{c^{-\frac{5}{6}}} \right)^{-\frac{3}{5}}} = \left(\frac{c^{\frac{1}{2} - \frac{1}{3}}}{c^{-\frac{5}{6}}} \right)^{-\frac{3}{5}} =$$

$$\underbrace{a^r \cdot a^s = a^{r+s}} \quad \underbrace{\frac{a^r}{a^s} = a^{r-s}} \quad \underbrace{(a^r)^s = a^{r \cdot s}}$$

$$\underbrace{\sqrt[r]{a} = a^{\frac{1}{r}}}$$

$$= \left(\frac{c^{\frac{1}{6}}}{c^{-\frac{5}{6}}} \right)^{-\frac{3}{5}} = \left(c^{\frac{1}{6} + \frac{5}{6}} \right)^{-\frac{3}{5}} = c^{-\frac{3}{5}} \quad \left| \begin{array}{l} c \neq 0 \\ c \geq 0 \\ \Downarrow \\ c > 0 \end{array} \right.$$

$$5) \left[\left(\frac{x}{y} \right)^2 - \frac{x}{y^2} \right] \cdot \left(\frac{x-1}{y} \right)^2 = \left(\frac{a}{b} \right)^r = \frac{a^r}{b^r}$$

$$= \left[\frac{x^2}{y^2} - \frac{x}{y} \right] \cdot \frac{(x-1)^2}{y^2} =$$

$$= \left(\frac{x^2 - x}{y} \right) \cdot \frac{1}{(x-1)^2} = \frac{x \cdot \cancel{(x-1)}}{(x-1)^2} = \frac{x}{x-1}$$

$$y \neq 0 \quad x-1 \neq 0 \rightarrow y \neq 0 \quad x \neq 1 \quad \checkmark$$

$$b) \frac{(\sqrt[4]{u} + \sqrt[4]{v})^2 + (\sqrt[4]{u} - \sqrt[4]{v})^2}{u - v} \cdot \frac{2}{\sqrt{u} - \sqrt{v}}$$

$$(A+B)^2 = A^2 + 2AB + B^2$$

$$(A-B)^2 = A^2 - 2AB + B^2$$

$$A = \sqrt[4]{u}$$

$$A^2 = \sqrt{u}$$

$$= \frac{2\sqrt{u} + 2\sqrt{v}}{u - v} \cdot \frac{\sqrt{u} - \sqrt{v}}{2}$$

$\underbrace{u - v}_{A^2 - B^2} \quad \underbrace{\sqrt{u} - \sqrt{v}}_{A - B}$

$$\begin{cases} u - v \neq 0 \\ u \geq 0 \\ v \geq 0 \end{cases}$$

$$= \frac{\cancel{2}(\cancel{\sqrt{u}} + \cancel{\sqrt{v}})}{\cancel{\sqrt{u}} + \cancel{\sqrt{v}}} \cdot \frac{1}{\cancel{2}} = 1$$

$$p(x) \quad p(x_i) = 0$$

$$= a_1 (x - x_1) \cdot (x - x_2) \dots$$

$$\frac{x-1}{x^2-2x+1} = \frac{\cancel{x-1}}{(x-1)^2} = \frac{1}{x-1}$$

$$ax^2 + bx + c = 0$$

$$x_{1,2} = \frac{-b \pm \sqrt{b^2 - 4ac}}{2a}$$

$$x^2 - 5x - 6 = 0$$

$$(x-6) \cdot (x+1) = 0$$

$$x_{1,2} = \frac{5 \pm \sqrt{25 + 24}}{2} = \frac{5 \pm 7}{2} = \begin{matrix} 6 \\ -1 \end{matrix}$$

$$\underline{x^2 - 5x - 6} = \left(x - \frac{5}{2}\right)^2 - 6 - \frac{25}{4} \quad \text{--- } B^2$$

$$(A+B)^2 = A^2 + 2A \cdot B + B^2 \quad A = x$$

$$2B = -5 \\ B = -\frac{5}{2}$$

$$= x^2 - 5x + \frac{25}{4} - 6 - \frac{25}{4}$$

$$\begin{aligned}
 x^2 - 5x - 6 &= \left(x - \frac{5}{2}\right)^2 - 6 - \frac{25}{4} \\
 &= \left(x - \frac{5}{2}\right)^2 - \frac{49}{4} \\
 &\quad \text{A}^2 - \text{B}^2 \quad D = \frac{7}{2} \\
 &= \left(x - \frac{5}{2} + \frac{7}{2}\right) \cdot \left(x - \frac{5}{2} - \frac{7}{2}\right) \\
 &= (x + 1)(x - 6)
 \end{aligned}$$

$$\underbrace{\sqrt{b^2 - 4ac}}_D \quad D < 0 \rightarrow \sqrt{D} \notin \mathbb{R}$$

$$x^2 + x + 1 = \left(x + \frac{1}{2}\right)^2 - \left(-\frac{3}{4}\right)$$

$$D = 1 - 4 = -3 \quad \text{A}^2 - \text{B}^2 \quad D^2 = -\frac{3}{4}$$

$$\times \quad (x - x_1)(x - x_2) \quad x_{1,2} \in \mathbb{R}$$

Trójčlenka

0,7 GB - 5 min.

4,9 GB - ? min

$$\begin{array}{l} \uparrow \quad 0,7 \text{ GB} \quad \dots \quad 5 \text{ min} \quad \uparrow \\ \uparrow \quad 4,9 \text{ GB} \quad \dots \quad x \quad \uparrow \end{array}$$

700 MB



GB

príklad
úmera

$$\frac{x}{5} = \frac{4,9}{0,7} \quad / \cdot 5$$

$$x = 7 \cdot 5 = 35 \text{ min}$$

Bázen

$$\begin{array}{l} \downarrow \quad 0,1 \text{ l/s} \quad \dots \quad 36 \text{ h} \quad \uparrow \\ \downarrow \quad 6 \text{ l/s} \quad \dots \quad x \quad \uparrow \end{array}$$

$$\frac{x}{36} = \frac{0,1}{6}$$

$$x = 0,6 \text{ h}$$

$$(a-b)(a^n + a^{n-1}b + \dots + ab^{n-1} + b^n) = a^{n+1} - b^{n+1}$$

$$n=3$$

$$(a-b)(a^3 + a^2b + ab^2 + b^3) = a^4 - b^4$$

$$17) \frac{\frac{a^3}{b^2} + \frac{a^2}{b} + a + b}{\frac{a^2}{b^2} - \frac{b^2}{a^2}} = \frac{\dots}{\frac{a^4 - b^4}{a^2 b^2}}$$

$$= \frac{a^2 b^2 \left(\frac{a^3}{b^2} + \frac{a^2}{b} + a + b \right)}{a^4 - b^4} = \frac{a^2 (a^3 + ab^2 + ab^2 + b^3)}{a^4 - b^4}$$

$$= \frac{a^2}{a-b}$$

$$\boxed{a, b \neq 0}$$

$$\frac{a^4 - b^4}{a^2 b^2} \neq 0$$

$$a^4 - b^4 \neq 0$$

$$(a^2 + b^2)(a^2 - b^2) \neq 0$$

$$a^2 \neq \pm b^2$$

$$a^2 \neq b^2$$

$$\boxed{a \neq \pm b}$$

$$\sqrt{4v^4 \sqrt{v^{12}}} = \sqrt{4} \sqrt{v^4 \sqrt{v^{12}}}$$

$$= 2 \left(v^4 v^{\frac{12}{2}} \right)^{\frac{1}{2}} = 2 \left(v^{4+6} \right)^{\frac{1}{2}}$$

$$= 2 \left(v^{10} \right)^{\frac{1}{2}}$$

$$= 2 v^{\frac{10}{2}} = \underline{2v^5}$$

$$v \geq 0$$